Lean4Axiomatic/Natural/Order.lean
@@ -2,7 +2,7 @@ import Lean4Axiomatic.Natural.Sign
 
 namespace ℕ
 
-class OrderBase (ℕ : Type) [AdditionBase ℕ] where
+class Order.Base (ℕ : Type) [Core ℕ] [Addition.Base ℕ] where
   leOp : LE ℕ := LE.mk λ n m => ∃ k : ℕ, n + k ≃ m
   le_defn {n m : ℕ} : n ≤ m ↔ ∃ k : ℕ, n + k ≃ m
 
@@ -10,10 +10,11 @@ class OrderBase (ℕ : Type) [AdditionBase ℕ] where
   lt_defn {n m : ℕ} : n < m ↔ n ≤ m ∧ n ≄ m
 
 -- Higher priority than the stdlib definitions
-attribute [instance default+1] OrderBase.leOp
-attribute [instance default+1] OrderBase.ltOp
+attribute [instance default+1] Order.Base.leOp
+attribute [instance default+1] Order.Base.ltOp
 
-class OrderProperties (ℕ : Type) [AdditionBase ℕ] extends OrderBase ℕ where
+class Order.Derived (ℕ : Type) [Core ℕ] [Addition.Base ℕ]
+    extends Order.Base ℕ where
   le_subst_step : AA.Substitutive (α := ℕ) step (· ≤ ·) (· ≤ ·)
   le_inject_step : AA.Injective (α := ℕ) step (· ≤ ·) (· ≤ ·)
   le_subst_eqv : AA.Substitutive₂ (α := ℕ) (· ≤ ·) (· ≃ ·) (· → ·)
@@ -34,61 +35,63 @@ class OrderProperties (ℕ : Type) [AdditionBase ℕ] extends OrderBase ℕ wher
   lt_split {n m : ℕ} : n < step m → n < m ∨ n ≃ m
   trichotomy {n m : ℕ} : AA.ExactlyOneOfThree (n < m) (n ≃ m) (n > m)
 
-attribute [instance] OrderProperties.le_subst_eqv
+attribute [instance] Order.Derived.le_subst_eqv
 
 namespace Derived
 
 variable {ℕ : Type}
+variable [Core ℕ]
+variable [Axioms.Derived ℕ]
+variable [Addition.Derived ℕ]
 
-instance [AdditionBase ℕ] : OrderBase ℕ where
+instance [Addition.Base ℕ] : Order.Base ℕ where
   le_defn {n m : ℕ} := Iff.intro id id
   lt_defn {n m : ℕ} := Iff.intro id id
 
-theorem le_subst_step
-    [AdditionBase ℕ] [OrderBase ℕ] {n₁ n₂ : ℕ}
+theorem le_subst_step [Order.Base ℕ] {n₁ n₂ : ℕ}
     : n₁ ≤ n₂ → step n₁ ≤ step n₂ := by
   intro (_ : n₁ ≤ n₂)
   show step n₁ ≤ step n₂
-  have ⟨d, (_ : n₁ + d ≃ n₂)⟩ := OrderBase.le_defn.mp ‹n₁ ≤ n₂›
-  apply OrderBase.le_defn.mpr
+  have ⟨d, (_ : n₁ + d ≃ n₂)⟩ := Order.Base.le_defn.mp ‹n₁ ≤ n₂›
+  apply Order.Base.le_defn.mpr
   exists d
   show step n₁ + d ≃ step n₂
   calc
     _ ≃ step n₁ + d := Eqv.refl
-    _ ≃ step (n₁ + d) := AdditionBase.step_add
+    _ ≃ step (n₁ + d) := Addition.step_add
     _ ≃ step n₂ := AA.subst ‹n₁ + d ≃ n₂›
 
-instance [AdditionBase ℕ] [OrderBase ℕ]
+instance [Order.Base ℕ]
     : AA.Substitutive (α := ℕ) step (· ≤ ·) (· ≤ ·) where
   subst := le_subst_step
 
 theorem le_inject_step
-    [AdditionBase ℕ] [OrderBase ℕ] {n₁ n₂ : ℕ}
+    [Order.Base ℕ] {n₁ n₂ : ℕ}
     : step n₁ ≤ step n₂ → n₁ ≤ n₂ := by
   intro (_ : step n₁ ≤ step n₂)
   show n₁ ≤ n₂
   have ⟨d, (_ : step n₁ + d ≃ step n₂)⟩ :=
-    OrderBase.le_defn.mp ‹step n₁ ≤ step n₂›
-  apply OrderBase.le_defn.mpr
+    Order.Base.le_defn.mp ‹step n₁ ≤ step n₂›
+  apply Order.Base.le_defn.mpr
   exists d
   show n₁ + d ≃ n₂
   have : step (n₁ + d) ≃ step n₂ := calc
     _ ≃ step (n₁ + d) := Eqv.refl
-    _ ≃ step n₁ + d := Eqv.symm AdditionBase.step_add
+    _ ≃ step n₁ + d := Eqv.symm Addition.step_add
     _ ≃ step n₂ := ‹step n₁ + d ≃ step n₂›
   exact AA.inject ‹step (n₁ + d) ≃ step n₂›
 
-instance [AdditionBase ℕ] [OrderBase ℕ]
+instance [Order.Base ℕ]
     : AA.Injective (α := ℕ) step (· ≤ ·) (· ≤ ·) where
   inject := le_inject_step
 
 theorem le_subst_eqv
-    [AdditionBase ℕ] [OrderBase ℕ] {n₁ n₂ m : ℕ}
+    [Order.Base ℕ] {n₁ n₂ m : ℕ}
     : n₁ ≃ n₂ → n₁ ≤ m → n₂ ≤ m := by
   intro (_ : n₁ ≃ n₂) (_ : n₁ ≤ m)
   show n₂ ≤ m
-  have ⟨d, (_ : n₁ + d ≃ m)⟩ := OrderBase.le_defn.mp ‹n₁ ≤ m›
-  apply OrderBase.le_defn.mpr
+  have ⟨d, (_ : n₁ + d ≃ m)⟩ := Order.Base.le_defn.mp ‹n₁ ≤ m›
+  apply Order.Base.le_defn.mpr
   exists d
   show n₂ + d ≃ m
   calc
@@ -96,95 +99,96 @@ theorem le_subst_eqv
     _ ≃ n₁ + d := Eqv.symm (AA.substL ‹n₁ ≃ n₂›)
     _ ≃ m      := ‹n₁ + d ≃ m›
 
-instance [AdditionBase ℕ] [OrderBase ℕ]
+instance [Order.Base ℕ]
     : AA.SubstitutiveForHand AA.Hand.L (α := ℕ) (· ≤ ·) (· ≃ ·) (· → ·) where
   subst₂ := le_subst_eqv
 
 theorem le_eqv_subst
-    [AdditionBase ℕ] [OrderBase ℕ] {n m₁ m₂ : ℕ}
+    [Order.Base ℕ] {n m₁ m₂ : ℕ}
     : m₁ ≃ m₂ → n ≤ m₁ → n ≤ m₂ := by
   intro (_ : m₁ ≃ m₂) (_ : n ≤ m₁)
   show n ≤ m₂
-  have ⟨d, (_ : n + d ≃ m₁)⟩ := OrderBase.le_defn.mp ‹n ≤ m₁›
-  apply OrderBase.le_defn.mpr
+  have ⟨d, (_ : n + d ≃ m₁)⟩ := Order.Base.le_defn.mp ‹n ≤ m₁›
+  apply Order.Base.le_defn.mpr
   exists d
   show n + d ≃ m₂
   exact Eqv.trans ‹n + d ≃ m₁› ‹m₁ ≃ m₂›
 
-instance [AdditionBase ℕ] [OrderBase ℕ]
+instance [Order.Base ℕ]
     : AA.SubstitutiveForHand AA.Hand.R (α := ℕ) (· ≤ ·) (· ≃ ·) (· → ·) where
   subst₂ := le_eqv_subst
 
-instance [AdditionBase ℕ] [OrderBase ℕ]
+instance [Order.Base ℕ]
     : AA.Substitutive₂ (α := ℕ) (· ≤ ·) (· ≃ ·) (· → ·) :=
   AA.Substitutive₂.mk
 
-theorem le_refl [AdditionBase ℕ] [OrderBase ℕ] {n : ℕ} : n ≤ n := by
-  apply OrderBase.le_defn.mpr
+theorem le_refl [Order.Base ℕ] {n : ℕ} : n ≤ n := by
+  apply Order.Base.le_defn.mpr
   exists (0 : ℕ)
   show n + 0 ≃ n
-  exact AdditionProperties.add_zero
+  exact Addition.add_zero
 
-instance [AdditionBase ℕ] [OrderBase ℕ] : Relation.Refl (α := ℕ) (· ≤ ·) where
+instance [Order.Base ℕ] : Relation.Refl (α := ℕ) (· ≤ ·) where
   refl := le_refl
 
 theorem le_step_split
-    [AdditionBase ℕ] [OrderBase ℕ] {n m : ℕ}
+    [Order.Base ℕ] {n m : ℕ}
     : n ≤ step m → n ≤ m ∨ n ≃ step m := by
   intro (_ : n ≤ step m)
   show n ≤ m ∨ n ≃ step m
-  have ⟨d, (_ : n + d ≃ step m)⟩ := OrderBase.le_defn.mp ‹n ≤ step m›
-  apply (cases_on (motive := λ x => d ≃ x → n ≤ m ∨ n ≃ step m) d · · Eqv.refl)
+  have ⟨d, (_ : n + d ≃ step m)⟩ := Order.Base.le_defn.mp ‹n ≤ step m›
+  let motive := λ x => d ≃ x → n ≤ m ∨ n ≃ step m
+  apply (Axioms.cases_on (motive := motive) d · · Eqv.refl)
   · intro (_ : d ≃ 0)
     apply Or.inr
     show n ≃ step m
     calc
       _ ≃ n      := Eqv.refl
-      _ ≃ n + 0  := Eqv.symm AdditionProperties.add_zero
+      _ ≃ n + 0  := Eqv.symm Addition.add_zero
       _ ≃ n + d  := Eqv.symm (AA.substR ‹d ≃ 0›)
       _ ≃ step m := ‹n + d ≃ step m›
   · intro e (_ : d ≃ step e)
     apply Or.inl
     show n ≤ m
-    apply OrderBase.le_defn.mpr
+    apply Order.Base.le_defn.mpr
     exists e
     show n + e ≃ m
     apply AA.inject (β := ℕ) (f := step) (rβ := (· ≃ ·))
     show step (n + e) ≃ step m
     calc
       _ ≃ step (n + e) := Eqv.refl
-      _ ≃ n + step e   := Eqv.symm AdditionProperties.add_step
+      _ ≃ n + step e   := Eqv.symm Addition.add_step
       _ ≃ n + d        := Eqv.symm (AA.substR ‹d ≃ step e›)
       _ ≃ step m       := ‹n + d ≃ step m›
 
 theorem le_step
-    [AdditionBase ℕ] [OrderBase ℕ] {n m : ℕ} : n ≤ m → n ≤ step m := by
+    [Order.Base ℕ] {n m : ℕ} : n ≤ m → n ≤ step m := by
   intro (_ : n ≤ m)
   show n ≤ step m
-  have ⟨d, (_ : n + d ≃ m)⟩ := OrderBase.le_defn.mp ‹n ≤ m›
-  apply OrderBase.le_defn.mpr
+  have ⟨d, (_ : n + d ≃ m)⟩ := Order.Base.le_defn.mp ‹n ≤ m›
+  apply Order.Base.le_defn.mpr
   exists step d
   show n + step d ≃ step m
   calc
     _ ≃ n + step d   := Eqv.refl
-    _ ≃ step (n + d) := AdditionProperties.add_step
+    _ ≃ step (n + d) := Addition.add_step
     _ ≃ step m       := AA.subst ‹n + d ≃ m›
 
 theorem le_trans
-    [AdditionBase ℕ] [OrderBase ℕ] {n m k : ℕ} : n ≤ m → m ≤ k → n ≤ k := by
+    [Order.Base ℕ] {n m k : ℕ} : n ≤ m → m ≤ k → n ≤ k := by
   intro (_ : n ≤ m)
-  have ⟨d, (_ : n + d ≃ m)⟩ := OrderBase.le_defn.mp ‹n ≤ m›
-  apply ind_on (motive := λ k => m ≤ k → n ≤ k) k
+  have ⟨d, (_ : n + d ≃ m)⟩ := Order.Base.le_defn.mp ‹n ≤ m›
+  apply Axioms.ind_on (motive := λ k => m ≤ k → n ≤ k) k
   case zero =>
     intro (_ : m ≤ 0)
-    have ⟨e, (_ : m + e ≃ 0)⟩ := OrderBase.le_defn.mp ‹m ≤ 0›
+    have ⟨e, (_ : m + e ≃ 0)⟩ := Order.Base.le_defn.mp ‹m ≤ 0›
     show n ≤ 0
-    apply OrderBase.le_defn.mpr
+    apply Order.Base.le_defn.mpr
     exists d + e
     show n + (d + e) ≃ 0
     calc
       _ ≃ n + (d + e) := Eqv.refl
-      _ ≃ (n + d) + e := Eqv.symm AdditionProperties.add_assoc
+      _ ≃ (n + d) + e := Eqv.symm Addition.add_assoc
       _ ≃ m + e       := AA.substL ‹n + d ≃ m›
       _ ≃ 0           := ‹m + e ≃ 0›
   case step =>
@@ -196,136 +200,136 @@ theorem le_trans
     | Or.inr (_ : m ≃ step k) =>
       exact AA.substR (rβ := (· → ·)) ‹m ≃ step k› ‹n ≤ m›
 
-instance [AdditionBase ℕ] [OrderBase ℕ] : Relation.Trans (α := ℕ) (· ≤ ·) where
+instance [Order.Base ℕ] : Relation.Trans (α := ℕ) (· ≤ ·) where
   trans := le_trans
 
 theorem le_subst_add
-    [AdditionBase ℕ] [OrderBase ℕ] {n₁ n₂ m : ℕ}
+    [Order.Base ℕ] {n₁ n₂ m : ℕ}
     : n₁ ≤ n₂ → n₁ + m ≤ n₂ + m := by
   intro (_ : n₁ ≤ n₂)
   show n₁ + m ≤ n₂ + m
-  have ⟨d, (_ : n₁ + d ≃ n₂)⟩ := OrderBase.le_defn.mp ‹n₁ ≤ n₂›
-  apply OrderBase.le_defn.mpr
+  have ⟨d, (_ : n₁ + d ≃ n₂)⟩ := Order.Base.le_defn.mp ‹n₁ ≤ n₂›
+  apply Order.Base.le_defn.mpr
   exists d
   show (n₁ + m) + d ≃ n₂ + m
   calc
     _ ≃ (n₁ + m) + d := Eqv.refl
-    _ ≃ n₁ + (m + d) := AdditionProperties.add_assoc
+    _ ≃ n₁ + (m + d) := Addition.add_assoc
     _ ≃ n₁ + (d + m) := AA.substR AA.comm
-    _ ≃ (n₁ + d) + m := Eqv.symm AdditionProperties.add_assoc
+    _ ≃ (n₁ + d) + m := Eqv.symm Addition.add_assoc
     _ ≃ n₂ + m       := AA.substL ‹n₁ + d ≃ n₂›
 
-instance [AdditionBase ℕ] [OrderBase ℕ]
+instance [Order.Base ℕ]
     : AA.SubstitutiveForHand AA.Hand.L (α := ℕ) (· + ·) (· ≤ ·) (· ≤ ·) where
   subst₂ := le_subst_add
 
-instance [AdditionBase ℕ] [OrderBase ℕ]
+instance [Order.Base ℕ]
     : AA.SubstitutiveForHand AA.Hand.R (α := ℕ) (· + ·) (· ≤ ·) (· ≤ ·) :=
   AA.substR_from_substL_swap
 
-instance [AdditionBase ℕ] [OrderBase ℕ]
+instance [Order.Base ℕ]
     : AA.Substitutive₂ (α := ℕ) (· + ·) (· ≤ ·) (· ≤ ·) :=
   AA.Substitutive₂.mk
 
 theorem le_cancel_add
-    [AdditionBase ℕ] [OrderBase ℕ] {n m₁ m₂ : ℕ}
+    [Order.Base ℕ] {n m₁ m₂ : ℕ}
     : n + m₁ ≤ n + m₂ → m₁ ≤ m₂ := by
   intro (_ : n + m₁ ≤ n + m₂)
   show m₁ ≤ m₂
   have ⟨d, (_ : (n + m₁) + d ≃ n + m₂)⟩ :=
-    OrderBase.le_defn.mp ‹n + m₁ ≤ n + m₂›
-  apply OrderBase.le_defn.mpr
+    Order.Base.le_defn.mp ‹n + m₁ ≤ n + m₂›
+  apply Order.Base.le_defn.mpr
   exists d
   show m₁ + d ≃ m₂
   have : n + (m₁ + d) ≃ n + m₂ := calc
     _ ≃ n + (m₁ + d) := Eqv.refl
-    _ ≃ (n + m₁) + d := Eqv.symm AdditionProperties.add_assoc
+    _ ≃ (n + m₁) + d := Eqv.symm Addition.add_assoc
     _ ≃ n + m₂       := ‹(n + m₁) + d ≃ n + m₂›
-  exact AdditionProperties.cancel_add ‹n + (m₁ + d) ≃ n + m₂›
+  exact Addition.cancel_add ‹n + (m₁ + d) ≃ n + m₂›
 
-instance [AdditionBase ℕ] [OrderBase ℕ]
+instance [Order.Base ℕ]
     : AA.Cancellative AA.Hand.L (α := ℕ) (· + ·) (· ≤ ·) (· ≤ ·) where
   cancel := le_cancel_add
 
-instance [AdditionBase ℕ] [OrderBase ℕ]
+instance [Order.Base ℕ]
     : AA.Cancellative AA.Hand.R (α := ℕ) (· + ·) (· ≤ ·) (· ≤ ·) :=
   AA.cancelR_from_cancelL
 
-instance [AdditionBase ℕ] [OrderBase ℕ]
+instance [Order.Base ℕ]
     : AA.Cancellative₂ (α := ℕ) (· + ·) (· ≤ ·) (· ≤ ·) := AA.Cancellative₂.mk
 
 theorem le_antisymm
-    [AdditionBase ℕ] [OrderBase ℕ] {n m : ℕ} : n ≤ m → m ≤ n → n ≃ m := by
+    [Order.Base ℕ] {n m : ℕ} : n ≤ m → m ≤ n → n ≃ m := by
   intro (_ : n ≤ m) (_ : m ≤ n)
   show n ≃ m
-  have ⟨d₁, (_ : n + d₁ ≃ m)⟩ := OrderBase.le_defn.mp ‹n ≤ m›
-  have ⟨d₂, (_ : m + d₂ ≃ n)⟩ := OrderBase.le_defn.mp ‹m ≤ n›
+  have ⟨d₁, (_ : n + d₁ ≃ m)⟩ := Order.Base.le_defn.mp ‹n ≤ m›
+  have ⟨d₂, (_ : m + d₂ ≃ n)⟩ := Order.Base.le_defn.mp ‹m ≤ n›
   have : n + (d₁ + d₂) ≃ n + 0 := calc
     _ ≃ n + (d₁ + d₂) := Eqv.refl
-    _ ≃ (n + d₁) + d₂ := Eqv.symm AdditionProperties.add_assoc
+    _ ≃ (n + d₁) + d₂ := Eqv.symm Addition.add_assoc
     _ ≃ m + d₂        := AA.substL ‹n + d₁ ≃ m›
     _ ≃ n             := ‹m + d₂ ≃ n›
-    _ ≃ n + 0         := Eqv.symm AdditionProperties.add_zero
-  have : d₁ + d₂ ≃ 0 := AdditionProperties.cancel_add ‹n + (d₁ + d₂) ≃ n + 0›
-  have ⟨(_ : d₁ ≃ 0), _⟩ := AdditionProperties.zero_sum_split ‹d₁ + d₂ ≃ 0›
+    _ ≃ n + 0         := Eqv.symm Addition.add_zero
+  have : d₁ + d₂ ≃ 0 := Addition.cancel_add ‹n + (d₁ + d₂) ≃ n + 0›
+  have ⟨(_ : d₁ ≃ 0), _⟩ := Addition.zero_sum_split ‹d₁ + d₂ ≃ 0›
   calc
     _ ≃ n      := Eqv.refl
-    _ ≃ n + 0  := Eqv.symm AdditionProperties.add_zero
+    _ ≃ n + 0  := Eqv.symm Addition.add_zero
     _ ≃ n + d₁ := Eqv.symm (AA.substR ‹d₁ ≃ 0›)
     _ ≃ m      := ‹n + d₁ ≃ m›
 
 theorem lt_subst_eqv
-    [AdditionBase ℕ] [OrderBase ℕ] {n₁ n₂ m : ℕ}
+    [Order.Base ℕ] {n₁ n₂ m : ℕ}
     : n₁ ≃ n₂ → n₁ < m → n₂ < m := by
   intro (_ : n₁ ≃ n₂) (_ : n₁ < m)
   show n₂ < m
-  have ⟨(_ : n₁ ≤ m), (_ : n₁ ≄ m)⟩ := OrderBase.lt_defn.mp ‹n₁ < m›
+  have ⟨(_ : n₁ ≤ m), (_ : n₁ ≄ m)⟩ := Order.Base.lt_defn.mp ‹n₁ < m›
   have : n₂ ≤ m := AA.substL (rβ := (· → ·)) ‹n₁ ≃ n₂› ‹n₁ ≤ m›
   have : n₂ ≄ m := AA.substL (f := (· ≄ ·)) (rβ := (· → ·)) ‹n₁ ≃ n₂› ‹n₁ ≄ m›
-  apply OrderBase.lt_defn.mpr
+  apply Order.Base.lt_defn.mpr
   exact ⟨‹n₂ ≤ m›, ‹n₂ ≄ m›⟩
 
-instance [AdditionBase ℕ] [OrderBase ℕ]
+instance [Order.Base ℕ]
     : AA.SubstitutiveForHand AA.Hand.L (α := ℕ) (· < ·) (· ≃ ·) (· → ·) where
   subst₂ := lt_subst_eqv
 
 theorem lt_eqv_subst
-    [AdditionBase ℕ] [OrderBase ℕ] {n₁ n₂ m : ℕ}
+    [Order.Base ℕ] {n₁ n₂ m : ℕ}
     : n₁ ≃ n₂ → m < n₁ → m < n₂ := by
   intro (_ : n₁ ≃ n₂) (_ : m < n₁)
   show m < n₂
-  have ⟨(_ : m ≤ n₁), (_ : m ≄ n₁)⟩ := OrderBase.lt_defn.mp ‹m < n₁›
+  have ⟨(_ : m ≤ n₁), (_ : m ≄ n₁)⟩ := Order.Base.lt_defn.mp ‹m < n₁›
   have : m ≤ n₂ := AA.substR (rβ := (· → ·)) ‹n₁ ≃ n₂› ‹m ≤ n₁›
   have : m ≄ n₂ := AA.substR (f := (· ≄ ·)) (rβ := (· → ·)) ‹n₁ ≃ n₂› ‹m ≄ n₁›
-  apply OrderBase.lt_defn.mpr
+  apply Order.Base.lt_defn.mpr
   exact ⟨‹m ≤ n₂›, ‹m ≄ n₂›⟩
 
-instance [AdditionBase ℕ] [OrderBase ℕ]
+instance [Order.Base ℕ]
     : AA.SubstitutiveForHand AA.Hand.R (α := ℕ) (· < ·) (· ≃ ·) (· → ·) where
   subst₂ := lt_eqv_subst
 
-instance [AdditionBase ℕ] [OrderBase ℕ]
+instance [Order.Base ℕ]
     : AA.Substitutive₂ (α := ℕ) (· < ·) (· ≃ ·) (· → ·) := AA.Substitutive₂.mk
 
-theorem lt_step [AdditionBase ℕ] [OrderBase ℕ] {n : ℕ} : n < step n := by
+theorem lt_step [Order.Base ℕ] {n : ℕ} : n < step n := by
   show n < step n
-  apply OrderBase.lt_defn.mpr
+  apply Order.Base.lt_defn.mpr
   apply And.intro
   · show n ≤ step n
-    apply OrderBase.le_defn.mpr
+    apply Order.Base.le_defn.mpr
     exists (1 : ℕ)
     show n + 1 ≃ step n
-    exact add_one_step
+    exact Addition.add_one_step
   · show n ≄ step n
     exact Eqv.symm Axioms.Derived.step_neq
 
 theorem lt_step_le
-    [AdditionBase ℕ] [OrderBase ℕ] {n m : ℕ} : n < m ↔ step n ≤ m := by
+    [Order.Base ℕ] {n m : ℕ} : n < m ↔ step n ≤ m := by
   apply Iff.intro
   · intro (_ : n < m)
     show step n ≤ m
-    have ⟨(_ : n ≤ m), (_ : n ≄ m)⟩ := OrderBase.lt_defn.mp ‹n < m›
-    have ⟨d, (_ : n + d ≃ m)⟩ := OrderBase.le_defn.mp ‹n ≤ m›
+    have ⟨(_ : n ≤ m), (_ : n ≄ m)⟩ := Order.Base.lt_defn.mp ‹n < m›
+    have ⟨d, (_ : n + d ≃ m)⟩ := Order.Base.le_defn.mp ‹n ≤ m›
     have : d ≄ 0 := by
       intro (_ : d ≃ 0)
       show False
@@ -333,31 +337,31 @@ theorem lt_step_le
       show n ≃ m
       calc
         _ ≃ n     := Eqv.refl
-        _ ≃ n + 0 := Eqv.symm AdditionProperties.add_zero
+        _ ≃ n + 0 := Eqv.symm Addition.add_zero
         _ ≃ n + d := Eqv.symm (AA.substR ‹d ≃ 0›)
         _ ≃ m     := ‹n + d ≃ m›
-    have : Positive d := SignBase.positive_defn.mpr ‹d ≄ 0›
-    have ⟨d', (_ : step d' ≃ d)⟩ := SignProperties.positive_step ‹Positive d›
+    have : Positive d := Sign.Base.positive_defn.mpr ‹d ≄ 0›
+    have ⟨d', (_ : step d' ≃ d)⟩ := Sign.Derived.positive_step ‹Positive d›
     show step n ≤ m
-    apply OrderBase.le_defn.mpr
+    apply Order.Base.le_defn.mpr
     exists d'
     show step n + d' ≃ m
     calc
       _ ≃ step n + d'   := Eqv.refl
-      _ ≃ step (n + d') := AdditionBase.step_add
-      _ ≃ n + step d'   := Eqv.symm AdditionProperties.add_step
+      _ ≃ step (n + d') := Addition.step_add
+      _ ≃ n + step d'   := Eqv.symm Addition.add_step
       _ ≃ n + d         := AA.substR ‹step d' ≃ d›
       _ ≃ m             := ‹n + d ≃ m›
   · intro (_ : step n ≤ m)
     show n < m
-    have ⟨d, (_ : step n + d ≃ m)⟩ := OrderBase.le_defn.mp ‹step n ≤ m›
+    have ⟨d, (_ : step n + d ≃ m)⟩ := Order.Base.le_defn.mp ‹step n ≤ m›
     have : n + step d ≃ m := calc
       _ ≃ n + step d   := Eqv.refl
-      _ ≃ step (n + d) := AdditionProperties.add_step
-      _ ≃ step n + d   := Eqv.symm AdditionBase.step_add
+      _ ≃ step (n + d) := Addition.add_step
+      _ ≃ step n + d   := Eqv.symm Addition.step_add
       _ ≃ m            := ‹step n + d ≃ m›
     have : ∃ d, n + d ≃ m := ⟨step d, ‹n + step d ≃ m›⟩
-    have : n ≤ m := OrderBase.le_defn.mpr ‹∃ d, n + d ≃ m›
+    have : n ≤ m := Order.Base.le_defn.mpr ‹∃ d, n + d ≃ m›
     have : n ≄ m := by
       intro (_ : n ≃ m)
       show False
@@ -365,52 +369,52 @@ theorem lt_step_le
         _ ≃ n + step d := Eqv.refl
         _ ≃ m := ‹n + step d ≃ m›
         _ ≃ n := Eqv.symm ‹n ≃ m›
-        _ ≃ n + 0 := Eqv.symm AdditionProperties.add_zero
-      have : step d ≃ 0 := AdditionProperties.cancel_add ‹n + step d ≃ n + 0›
+        _ ≃ n + 0 := Eqv.symm Addition.add_zero
+      have : step d ≃ 0 := Addition.cancel_add ‹n + step d ≃ n + 0›
       exact absurd this Axioms.step_neq_zero
     show n < m
-    apply OrderBase.lt_defn.mpr
+    apply Order.Base.lt_defn.mpr
     exact ⟨‹n ≤ m›, ‹n ≄ m›⟩
 
-theorem lt_zero [AdditionBase ℕ] [OrderBase ℕ] {n : ℕ} : n ≮ 0 := by
+theorem lt_zero [Order.Base ℕ] {n : ℕ} : n ≮ 0 := by
   intro (_ : n < 0)
   show False
   have : step n ≤ 0 := lt_step_le.mp ‹n < 0›
-  have ⟨d, (_ : step n + d ≃ 0)⟩ := OrderBase.le_defn.mp ‹step n ≤ 0›
+  have ⟨d, (_ : step n + d ≃ 0)⟩ := Order.Base.le_defn.mp ‹step n ≤ 0›
   have : step (n + d) ≃ 0 := calc
     _ ≃ step (n + d) := Eqv.refl
-    _ ≃ step n + d   := Eqv.symm AdditionBase.step_add
+    _ ≃ step n + d   := Eqv.symm Addition.step_add
     _ ≃ 0            := ‹step n + d ≃ 0›
   exact absurd ‹step (n + d) ≃ 0› Axioms.step_neq_zero
 
 theorem le_from_eqv
-    [AdditionBase ℕ] [OrderBase ℕ] {n m : ℕ} : n ≃ m → n ≤ m := by
+    [Order.Base ℕ] {n m : ℕ} : n ≃ m → n ≤ m := by
   intro (_ : n ≃ m)
   show n ≤ m
   have : n ≤ n := Eqv.refl
   exact AA.substR (rβ := (· → ·)) ‹n ≃ m› ‹n ≤ n›
 
 theorem le_from_lt
-    [AdditionBase ℕ] [OrderBase ℕ] {n m : ℕ} : n < m → n ≤ m := by
+    [Order.Base ℕ] {n m : ℕ} : n < m → n ≤ m := by
   intro (_ : n < m)
   show n ≤ m
-  have ⟨(_ : n ≤ m), _⟩ := OrderBase.lt_defn.mp ‹n < m›
+  have ⟨(_ : n ≤ m), _⟩ := Order.Base.lt_defn.mp ‹n < m›
   exact ‹n ≤ m›
 
 theorem le_split
-    [AdditionBase ℕ] [OrderBase ℕ] {n m : ℕ} : n ≤ m → n < m ∨ n ≃ m := by
+    [Order.Base ℕ] {n m : ℕ} : n ≤ m → n < m ∨ n ≃ m := by
   intro (_ : n ≤ m)
   show n < m ∨ n ≃ m
-  have ⟨d, (h : n + d ≃ m)⟩ := OrderBase.le_defn.mp ‹n ≤ m›
+  have ⟨d, (h : n + d ≃ m)⟩ := Order.Base.le_defn.mp ‹n ≤ m›
   revert h
-  apply cases_on (motive := λ d => n + d ≃ m → n < m ∨ n ≃ m) d
+  apply Axioms.cases_on (motive := λ d => n + d ≃ m → n < m ∨ n ≃ m) d
   case zero =>
     intro (_ : n + 0 ≃ m)
     apply Or.inr
     show n ≃ m
     calc
       _ ≃ n     := Eqv.refl
-      _ ≃ n + 0 := Eqv.symm add_zero
+      _ ≃ n + 0 := Eqv.symm Addition.add_zero
       _ ≃ m     := ‹n + 0 ≃ m›
   case step =>
     intro d (_ : n + step d ≃ m)
@@ -418,17 +422,17 @@ theorem le_split
     show n < m
     apply lt_step_le.mpr
     show step n ≤ m
-    apply OrderBase.le_defn.mpr
+    apply Order.Base.le_defn.mpr
     exists d
     show step n + d ≃ m
     calc
       _ ≃ step n + d   := Eqv.refl
-      _ ≃ step (n + d) := AdditionBase.step_add
-      _ ≃ n + step d   := Eqv.symm add_step
+      _ ≃ step (n + d) := Addition.step_add
+      _ ≃ n + step d   := Eqv.symm Addition.add_step
       _ ≃ m            := ‹n + step d ≃ m›
 
 theorem lt_split
-    [AdditionBase ℕ] [OrderBase ℕ] {n m : ℕ} : n < step m → n < m ∨ n ≃ m := by
+    [Order.Base ℕ] {n m : ℕ} : n < step m → n < m ∨ n ≃ m := by
   intro (_ : n < step m)
   show n < m ∨ n ≃ m
   have : step n ≤ step m := lt_step_le.mp ‹n < step m›
@@ -436,7 +440,7 @@ theorem lt_split
   exact le_split ‹n ≤ m›
 
 theorem lt_trans
-    [AdditionBase ℕ] [OrderBase ℕ] {n m k : ℕ} : n < m → m < k → n < k := by
+    [Order.Base ℕ] {n m k : ℕ} : n < m → m < k → n < k := by
   intro (_ : n < m) (_ : m < k)
   show n < k
   apply lt_step_le.mpr
@@ -447,19 +451,19 @@ theorem lt_trans
     _ ≤ step m := le_from_lt lt_step
     _ ≤ k      := lt_step_le.mp ‹m < k›
 
-instance [AdditionBase ℕ] [OrderBase ℕ]: Relation.Trans (α := ℕ) (· < ·) where
+instance [Order.Base ℕ]: Relation.Trans (α := ℕ) (· < ·) where
   trans := lt_trans
 
 theorem trichotomy
-    [AdditionBase ℕ] [OrderBase ℕ] {n m : ℕ}
+    [Order.Base ℕ] {n m : ℕ}
     : AA.ExactlyOneOfThree (n < m) (n ≃ m) (n > m) := by
   constructor
   case atLeastOne =>
-    apply ind_on (motive := λ n => AA.OneOfThree (n < m) (n ≃ m) (n > m)) n
+    apply Axioms.ind_on (motive := λ n => AA.OneOfThree (n < m) (n ≃ m) (n > m)) n
     case zero =>
       show AA.OneOfThree (0 < m) (0 ≃ m) (0 > m)
-      apply cases_on
-        (motive := λ m : ℕ => AA.OneOfThree (0 < m) (0 ≃ m) (0 > m)) m
+      let motive := λ m : ℕ => AA.OneOfThree (0 < m) (0 ≃ m) (0 > m)
+      apply Axioms.cases_on (motive := motive) m
       case zero =>
         apply AA.OneOfThree.second
         show 0 ≃ 0
@@ -468,12 +472,12 @@ theorem trichotomy
         intro m
         apply AA.OneOfThree.first
         show 0 < step m
-        apply OrderBase.lt_defn.mpr
+        apply Order.Base.lt_defn.mpr
         apply And.intro
         · show 0 ≤ step m
-          apply OrderBase.le_defn.mpr
+          apply Order.Base.le_defn.mpr
           exists step m
-          exact AdditionBase.zero_add
+          exact Addition.zero_add
         · show 0 ≄ step m
           exact Eqv.symm Axioms.step_neq_zero
     case step =>
@@ -502,20 +506,20 @@ theorem trichotomy
     intro
     | AA.TwoOfThree.oneAndTwo (_ : n < m) (_ : n ≃ m) =>
       show False
-      have ⟨_, (_ : n ≄ m)⟩ := OrderBase.lt_defn.mp ‹n < m›
+      have ⟨_, (_ : n ≄ m)⟩ := Order.Base.lt_defn.mp ‹n < m›
       exact absurd ‹n ≃ m› ‹n ≄ m›
     | AA.TwoOfThree.oneAndThree (_ : n < m) (_ : n > m) =>
       show False
-      have ⟨(_ : n ≤ m), (_ : n ≄ m)⟩ := OrderBase.lt_defn.mp ‹n < m›
-      have ⟨(_ : m ≤ n), _⟩ := OrderBase.lt_defn.mp ‹n > m›
+      have ⟨(_ : n ≤ m), (_ : n ≄ m)⟩ := Order.Base.lt_defn.mp ‹n < m›
+      have ⟨(_ : m ≤ n), _⟩ := Order.Base.lt_defn.mp ‹n > m›
       have : n ≃ m := le_antisymm ‹n ≤ m› ‹m ≤ n›
       exact absurd ‹n ≃ m› ‹n ≄ m›
     | AA.TwoOfThree.twoAndThree (_ : n ≃ m) (_ : n > m) =>
       show False
-      have ⟨_, (_ : m ≄ n)⟩ := OrderBase.lt_defn.mp ‹n > m›
+      have ⟨_, (_ : m ≄ n)⟩ := Order.Base.lt_defn.mp ‹n > m›
       exact absurd ‹n ≃ m› (Eqv.symm ‹m ≄ n›)
 
-instance [AdditionBase ℕ] : OrderProperties ℕ where
+instance : Order.Derived ℕ where
   le_subst_step := inferInstance
   le_inject_step := inferInstance
   le_subst_eqv := inferInstance
