Lean4Axiomatic/Natural/Sign.lean
@@ -2,47 +2,49 @@ import Lean4Axiomatic.Natural.Addition
 
 namespace ℕ
 
-class SignBase (ℕ : Type) [Constructors ℕ] [Equality ℕ] where
+class Sign.Base (ℕ : Type) [Core ℕ] where
   Positive (n : ℕ) : Prop := n ≄ 0
   positive_defn {n : ℕ} : Positive n ↔ n ≄ 0
 
-export SignBase (Positive)
-
-class SignProperties (ℕ : Type) [AdditionBase ℕ] extends SignBase ℕ where
+class Sign.Derived (ℕ : Type) [Core ℕ] [Addition.Base ℕ]
+    extends Sign.Base ℕ where
   positive_subst : AA.Substitutive Positive (· ≃ ·) (· → ·)
   positive_step {n : ℕ} : Positive n → ∃ m : ℕ, step m ≃ n
   positive_add {n m : ℕ} : Positive n → Positive (n + m)
 
+export Sign.Base (Positive)
+
 namespace Derived
 
 variable {ℕ : Type}
+variable [Core ℕ]
 
-instance [Constructors ℕ] [Equality ℕ] : SignBase ℕ where
+instance : Sign.Base ℕ where
   positive_defn := Iff.intro id id
 
 theorem positive_subst
-    [Constructors ℕ] [Equality ℕ] [SignBase ℕ] {n₁ n₂ : ℕ}
-    : n₁ ≃ n₂ → Positive n₁ → Positive n₂ := by
+    [Sign.Base ℕ] {n₁ n₂ : ℕ} : n₁ ≃ n₂ → Positive n₁ → Positive n₂ := by
   intro (_ : n₁ ≃ n₂) (_ : Positive n₁)
   show Positive n₂
-  have : n₁ ≄ 0 := SignBase.positive_defn.mp ‹Positive n₁›
-  apply SignBase.positive_defn.mpr
+  have : n₁ ≄ 0 := Sign.Base.positive_defn.mp ‹Positive n₁›
+  apply Sign.Base.positive_defn.mpr
   show n₂ ≄ 0
   exact AA.substL (self := AA.neq.substL) ‹n₁ ≃ n₂› ‹n₁ ≄ 0›
 
 instance
-    [Constructors ℕ] [Equality ℕ] [SignBase ℕ]
+    [Core ℕ] [Sign.Base ℕ]
     : AA.Substitutive (α := ℕ) Positive (· ≃ ·) (· → ·) where
   subst := positive_subst
 
 theorem positive_step
-    [Axioms ℕ] [SignBase ℕ] {n : ℕ} : Positive n → ∃ m : ℕ, step m ≃ n := by
-  apply cases_on (motive := λ n => Positive n → ∃ m, step m ≃ n) n
+    [Axioms.Derived ℕ] [Sign.Base ℕ] {n : ℕ}
+    : Positive n → ∃ m : ℕ, step m ≃ n := by
+  apply Axioms.cases_on (motive := λ n => Positive n → ∃ m, step m ≃ n) n
   case zero =>
     intro (_ : Positive (0 : ℕ))
     apply False.elim
     show False
-    have : 0 ≄ 0 := SignBase.positive_defn.mp ‹Positive (0 : ℕ)›
+    have : 0 ≄ 0 := Sign.Base.positive_defn.mp ‹Positive (0 : ℕ)›
     apply this
     show 0 ≃ 0
     exact Eqv.refl
@@ -53,25 +55,27 @@ theorem positive_step
     exact Eqv.refl
 
 theorem positive_add
-    [AdditionBase ℕ] [SignBase ℕ] {n m : ℕ}
+    [Axioms.Derived ℕ] [Addition.Derived ℕ] [Sign.Base ℕ] {n m : ℕ}
     : Positive n → Positive (n + m) := by
   intro (_ : Positive n)
   show Positive (n + m)
-  apply cases_on (motive := λ m => Positive (n + m)) m
+  apply Axioms.cases_on (motive := λ m => Positive (n + m)) m
   case zero =>
     show Positive (n + 0)
-    apply AA.subst (rβ := (· → ·)) (Eqv.symm AdditionProperties.add_zero)
+    apply AA.subst (rβ := (· → ·)) (Eqv.symm Addition.add_zero)
     exact ‹Positive n›
   case step =>
     intro m
     show Positive (n + step m)
-    apply AA.subst (rβ := (· → ·)) (Eqv.symm AdditionProperties.add_step)
+    apply AA.subst (rβ := (· → ·)) (Eqv.symm Addition.add_step)
     show Positive (step (n + m))
-    apply SignBase.positive_defn.mpr
+    apply Sign.Base.positive_defn.mpr
     show step (n + m) ≄ 0
     exact Axioms.step_neq_zero
 
-instance signProperties [AdditionBase ℕ] [SignBase ℕ] : SignProperties ℕ where
+instance signProperties
+    [Axioms.Derived ℕ] [Addition.Derived ℕ] [Sign.Base ℕ]
+    : Sign.Derived ℕ where
   positive_subst := inferInstance
   positive_step := positive_step
   positive_add := positive_add
